\documentclass[../main.tex]{subfiles}

\begin{document}

\problem{2}
Find the angle between the following pairs of vectors.
\begin{enumerate}[a)]
	\setcounter{enumi}{1}
	\item
		$\vec{u} = \begin{bmatrix}3&-1&0\end{bmatrix}^T$,
		$\vec{v} = \begin{bmatrix}-6&2&0\end{bmatrix}^T$
\end{enumerate}

\solution
\begin{enumerate}[a)]
	\setcounter{enumi}{1}
	\item Let $\theta$ be the angle.
		Compute the dot product of the vectors
		\[
			\vec{u}\cdot\vec{v}
			=
			3\cdot(-6) + (-1)\cdot2 + 0\cdot0
			=
			-18 - 2
			=
			-20
		\]
		and observe that as a consequence of it being negative, the angle between them is obtuse.
		Now compute the lengths of the vectors
		\[
			\|\vec{u}\| = \sqrt{3^2 + (-1)^2 + 0^2} = \sqrt{9 + 1 + 0} = \sqrt{10}
		\]
		\[
			\|\vec{v}\| = \sqrt{(-6)^2 + 2^2 + 0^2} = \sqrt{36 + 40 + 0} = \sqrt{40}
		\]
		and use these values to calculate the angle
		\begin{align*}
		\theta &= \cos^{-1}\left(\frac{\vec{u}\cdot\vec{v}}{\|\vec{u}\|\|\vec{v}\|}\right)
			\\
			&= \cos^{-1}\left(\frac{-20}{\sqrt{10}\sqrt{40}}\right)
			\\
			&= \cos^{-1}\left(\frac{-20}{\sqrt{400}}\right)
			\\
			&= \cos^{-1}\left(\frac{-20}{20}\right)
			\\
			&= \cos^{-1}\left(-1\right)
		\end{align*}
		which tells us that the angle between the two vectors is $\pi$. This is easily confirmed, as \(\vec{v} = -2\vec{u}\).
\end{enumerate}

\end{document}
