\documentclass[../main.tex]{subfiles}

\begin{document}

\problem{3}
If $T: \RR^2 \to \RR^2$ is as in $(b)$ and $(d)$ of Exercise 1, find $T\left(\begin{bmatrix}1&1\end{bmatrix}^T\right)$ and $T\left(\begin{bmatrix}2&-1\end{bmatrix}^T\right)$.

\solution
\begin{enumerate}[a)]
	\setcounter{enumi}{1}
	\item 
		\[
			%T\left(\begin{bmatrix}1&1\end{bmatrix}^T\right)
			%=
			\begin{bmatrix*}[r]0&-1\\-1&0\end{bmatrix*}
			\begin{bmatrix}1\\1\end{bmatrix}
			=
			\begin{bmatrix}
				0\cdot1 + (-1)\cdot1 \\
				(-1)\cdot1 + 0\cdot1
			\end{bmatrix}
			=
			\begin{bmatrix}
				0 - 1 \\
				(-1) + 0
			\end{bmatrix}
			=
			\begin{bmatrix}
				-1 \\
				-1
			\end{bmatrix}
		\]
		\[
			%T\left(\begin{bmatrix}2&-1\end{bmatrix}^T\right)
			%=
			\begin{bmatrix*}[r]0&-1\\-1&0\end{bmatrix*}
			\begin{bmatrix*}[r]2\\-1\end{bmatrix*}
			=
			\begin{bmatrix}
				0\cdot2 + (-1)\cdot(-1) \\
				(-1)\cdot2 + 0\cdot(-1)
			\end{bmatrix}
			=
			\begin{bmatrix}
				0 + 1 \\
				(-2) + 0
			\end{bmatrix}
			=
			\begin{bmatrix*}[r]
				1 \\
				-2
			\end{bmatrix*}
		\]
	\setcounter{enumi}{3}
	\item 
		\[
			\begin{bmatrix*}[r]0&1\\-1&0\end{bmatrix*}
			\begin{bmatrix}1\\1\end{bmatrix}
			=
			\begin{bmatrix}
				0\cdot1 + 1\cdot1 \\
				(-1)\cdot1 + 0\cdot1
			\end{bmatrix}
			=
			\begin{bmatrix}
				0 + 1 \\
				(-1) + 0
			\end{bmatrix}
			=
			\begin{bmatrix*}[r]
				1 \\
				-1
			\end{bmatrix*}
		\]
		\[
			\begin{bmatrix*}[r]0&1\\-1&0\end{bmatrix*}
			\begin{bmatrix*}[r]2\\-1\end{bmatrix*}
			=
			\begin{bmatrix}
				0\cdot2 + 1\cdot(-1) \\
				(-1)\cdot2 + 0\cdot(-1)
			\end{bmatrix}
			=
			\begin{bmatrix}
				0 - 1 \\
				(-2) + 0
			\end{bmatrix}
			=
			\begin{bmatrix*}[r]
				-1 \\
				-2
			\end{bmatrix*}
		\]
\end{enumerate}

\end{document}
