\documentclass[../main.tex]{subfiles}

\begin{document}

\problem{11}
Let
$\vec{u} = \begin{bmatrix}3&-1&0\end{bmatrix}^T$,
$\vec{v} = \begin{bmatrix}4&0&1\end{bmatrix}^T$, and
$\vec{w} = \begin{bmatrix}-1&1&5\end{bmatrix}^T$.
In each case, find $\vec{x}$ such that:
\begin{enumerate}[a)]
	\setcounter{enumi}{1}
	\item $2(3\vec{v} - \vec{x}) = 5\vec{w} + \vec{u} - 3\vec{x}$
\end{enumerate}

\solution
\begin{enumerate}[a)]
	\setcounter{enumi}{1}
	\item 
		\begin{align*}
			&& 2(3\vec{v} - \vec{x}) &= 5\vec{w} + \vec{u} - 3\vec{x} \\
			\Rightarrow && 6\vec{v} - 2\vec{x} &= 5\vec{w} + \vec{u} - 3\vec{x} \\
			\Rightarrow && 3\vec{x} - 2\vec{x} &= 5\vec{w} + \vec{u} - 6\vec{v} \\
			\Rightarrow && \vec{x} &= 5\vec{w} + \vec{u} - 6\vec{v} \\
			\Rightarrow && \vec{x} &= 5\begin{bmatrix*}[r]-1\\1\\5\end{bmatrix*} + \begin{bmatrix*}[r]3\\-1\\0\end{bmatrix*} - 6\begin{bmatrix}4\\0\\1\end{bmatrix} \\
			\Rightarrow && \vec{x} &= \begin{bmatrix*}[r]-5\\5\\25\end{bmatrix*} + \begin{bmatrix*}[r]3\\-1\\0\end{bmatrix*} - \begin{bmatrix}24\\0\\6\end{bmatrix} \\
			\Rightarrow && \vec{x} &= \begin{bmatrix}-5 + 3 - 24\\5 - 1\\25 - 6\end{bmatrix} \\
			\Rightarrow && \vec{x} &= \begin{bmatrix*}[r]-26\\4\\19\end{bmatrix*} \\
		\end{align*}
\end{enumerate}

\end{document}
