\documentclass[../main.tex]{subfiles}

\begin{document}

\problem{5}
\begin{enumerate}[a)]
	\setcounter{enumi}{1}
	\item 
		\begin{align*}
			-2x + 3y + 3z &= -9 \\
			3x - 4y + z &= 5 \\
			-5x + 7y + 2z &= -14
		\end{align*}
	\setcounter{enumi}{3}
	\item 
		\begin{align*}
			x + 2y - z &= 2 \\
			2x + 5y - 3z &= 1 \\
			x + 4y - 3z &= 3
		\end{align*}
	\setcounter{enumi}{5}
	\item 
		\begin{align*}
			3x - 2y + z &= -2 \\
			x - y + 3z &= 5 \\
			-x + y + z &= -1
		\end{align*}
\end{enumerate}

\solution
\begin{enumerate}[a)]
	\setcounter{enumi}{1}
	\item 
		Take the system of equations
		\begin{align*}
			-2x + 3y + 3z &= -9 \\
			3x - 4y + z &= 5 \\
			-5x + 7y + 2z &= -14
		\end{align*}
		Translate them to augmented matrix
		$$\left[\begin{array}{ccc|c}
			-2 & 3 & 3 & -9 \\
			3 & -4 & 1 & 5 \\
			-5 & 7 & 2 & -14
		\end{array}\right]$$
		Add the first row to the second
		$$\left[\begin{array}{ccc|c}
			-2 & 3 & 3 & -9 \\
			1 & -1 & 4 & -4 \\
			-5 & 7 & 2 & -14
		\end{array}\right]$$
		Swap the first and second row
		$$\left[\begin{array}{ccc|c}
			1 & -1 & 4 & -4 \\
			-2 & 3 & 3 & -9 \\
			-5 & 7 & 2 & -14
		\end{array}\right]$$
		Add the first row to the second twice
		$$\left[\begin{array}{ccc|c}
			1 & -1 & 4 & -4 \\
			0 & 1 & 11 & -17 \\
			-5 & 7 & 2 & -14
		\end{array}\right]$$
		Add the first row to the third five times
		$$\left[\begin{array}{ccc|c}
			1 & -1 & 4 & -4 \\
			0 & 1 & 11 & -17 \\
			0 & 2 & 22 & -34
		\end{array}\right]$$
		Subtract the second row from the third twice
		$$\left[\begin{array}{ccc|c}
			1 & -1 & 4 & -4 \\
			0 & 1 & 11 & -17 \\
			0 & 0 & 00 & 0
		\end{array}\right]$$
		Add the second row to the first
		$$\left[\begin{array}{ccc|c}
			1 & 0 & 15 & -21 \\
			0 & 1 & 11 & -17 \\
			0 & 0 & 00 & 0
		\end{array}\right]$$
		Let $z = t$, then it along with $x = -15t - 21$ and $y = -11t - 17$ form infinite solutions to the system of equations.
	\setcounter{enumi}{3}
	\item 
		Take the system of equations
		\begin{align*}
			x + 2y - z &= 2 \\
			2x + 5y - 3z &= 1 \\
			x + 4y - 3z &= 3
		\end{align*}
		Translate them to augmented matrix
		$$\left[\begin{array}{ccc|c}
			1 & 2 & -1 & 2 \\
			2 & 5 & -3 & 1 \\
			1 & 4 & -3 & 3
		\end{array}\right]$$
		Subtract the first row from the second row twice
		$$\left[\begin{array}{ccc|c}
			1 & 2 & -1 & 2 \\
			0 & 1 & -1 & -3 \\
			1 & 4 & -3 & 3
		\end{array}\right]$$
		Subtract the first row from the third row
		$$\left[\begin{array}{ccc|c}
			1 & 2 & -1 & 2 \\
			0 & 1 & -1 & -3 \\
			0 & 2 & -2 & 1
		\end{array}\right]$$
		Subtract the second row from the third row twice
		$$\left[\begin{array}{ccc|c}
			1 & 2 & -1 & 2 \\
			0 & 1 & -1 & -3 \\
			0 & 0 & 0 & 5
		\end{array}\right]$$
		Multiply the third row by a fifth
		$$\left[\begin{array}{ccc|c}
			1 & 2 & -1 & 2 \\
			0 & 1 & -1 & -3 \\
			0 & 0 & 0 & 1
		\end{array}\right]$$
		Since we have encountered a row of the form $\left[\begin{array}{ccc|c}0&\cdots&0&1\end{array}\right]$, the system of equations is inconsistent and therefore there is no solution.
	\setcounter{enumi}{5}
	\item 
		Take the system of equations
		\begin{align*}
			3x - 2y + z &= -2 \\
			x - y + 3z &= 5 \\
			-x + y + z &= -1
		\end{align*}
		Translate them to augmented matrix
		$$\left[\begin{array}{ccc|c}
			3 & -2 & 1 & -2 \\
			1 & -1 & 3 & 5 \\
			-1 & 1 & 1 & -1
		\end{array}\right]$$
		Swap the first and second row
		$$\left[\begin{array}{ccc|c}
			1 & -1 & 3 & 5 \\
			3 & -2 & 1 & -2 \\
			-1 & 1 & 1 & -1
		\end{array}\right]$$
		Subtract the first row from the second thrice
		$$\left[\begin{array}{ccc|c}
			1 & -1 & 3 & 5 \\
			0 & 1 & -8 & -17 \\
			-1 & 1 & 1 & -1
		\end{array}\right]$$
		Add the first row to the third
		$$\left[\begin{array}{ccc|c}
			1 & -1 & 3 & 5 \\
			0 & 1 & -8 & -17 \\
			0 & 0 & 4 & 4
		\end{array}\right]$$
		Multiply the third row by a fourth
		$$\left[\begin{array}{ccc|c}
			1 & -1 & 3 & 5 \\
			0 & 1 & -8 & -17 \\
			0 & 0 & 1 & 1
		\end{array}\right]$$
		From this we have that $z = 1$.
		We also see that
		\begin{align*}
			&& y - 8z &= -17 \\
			\Rightarrow && y &= 8z - 17 \\
			\Rightarrow && y &= 8 - 17 \\
			\Rightarrow && y &= -9 \\
		\end{align*}
		and
		\begin{align*}
			&& x - y + 3z &= 5 \\
			\Rightarrow && x &= y - 3z + 5 \\
			\Rightarrow && x &= -9 - 3 + 5 \\
			\Rightarrow && x &= -7
		\end{align*}
		so $x = -7$, $y = -9$, and $z = 1$ form a unique solution to the system of equations.
\end{enumerate}

\end{document}
