
%
% Worked by Ragnar Ardal
%
% Page numbers:
%  -    p - 7th Custom Edition
%  -  230 - Icelandic Edition
%  -    p - 7th Edition (US)
%  -    p - 6th Edition
%  -    p - 7th Global Edition
%

\problem{15}
	Let
	$$\mathbf{A} = \begin{bmatrix} 1 & 1 \\ 1 & 1 \end{bmatrix}.$$
	Find a formula for $\mathbf{A}^n$,
	whenever $n$ is a positive integer.

\solution
	$$\mathbf{A}^2 = \mathbf{A} \cdot \mathbf{A}
	               = \begin{bmatrix} 1 & 1 \\ 1 & 1 \end{bmatrix}\cdot\begin{bmatrix} 1 & 1 \\ 1 & 1 \end{bmatrix}
	               = \begin{bmatrix} (1 \cdot 1) + (1 \cdot 1) & (1 \cdot 1) + (1 \cdot 1) \\ (1 \cdot 1) + (1 \cdot 1) & (1 \cdot 1) + (1 \cdot 1) \end{bmatrix}
	               = \begin{bmatrix} 2 & 2 \\ 2 & 2 \end{bmatrix}
	$$

	$$\mathbf{A}^3 = \mathbf{A}^2 \cdot \mathbf{A}
	               = \begin{bmatrix} 2 & 2 \\ 2 & 2 \end{bmatrix}\cdot\begin{bmatrix} 1 & 1 \\ 1 & 1 \end{bmatrix}
	               = \begin{bmatrix} (2 \cdot 1) + (2 \cdot 1) & (2 \cdot 1) + (2 \cdot 1) \\ (2 \cdot 1) + (2 \cdot 1) & (2 \cdot 1) + (2 \cdot 1) \end{bmatrix}
	               = \begin{bmatrix} 4 & 4 \\ 4 & 4 \end{bmatrix}
	$$

	$$\mathbf{A}^4 = \mathbf{A}^3 \cdot \mathbf{A}
	               = \begin{bmatrix} 4 & 4 \\ 4 & 4 \end{bmatrix}\cdot\begin{bmatrix} 1 & 1 \\ 1 & 1 \end{bmatrix}
	               = \begin{bmatrix} (4 \cdot 1) + (4 \cdot 1) & (4 \cdot 1) + (4 \cdot 1) \\ (4 \cdot 1) + (4 \cdot 1) & (4 \cdot 1) + (4 \cdot 1) \end{bmatrix}
	               = \begin{bmatrix} 8 & 8 \\ 8 & 8 \end{bmatrix}
	$$

	$$\mathbf{A}^n = \begin{bmatrix} 2^{n-1} & 2^{n-1} \\ 2^{n-1} & 2^{n-1} \end{bmatrix}
	$$

	We can prove this formula with induction.
